\documentclass[a4paper,10pt]{article}
\usepackage{amssymb}
\usepackage{amsmath}
\usepackage[utf8]{inputenc}
\title{FDTD 1D with CPML}
\author{skiloop(skiloop@126.com)}
\begin{document}
\maketitle
\section{Maxwell Eqations}
Equations in frequancy domain
\begin{equation}
j\omega\epsilon E_{x}=-\frac{1}{s_{z}}\frac{\partial H_{y}}{\partial z}
\end{equation}
\begin{equation}
j\omega\mu H_{y}=\frac{1}{s_{z}}\frac{\partial E_{x}}{\partial z}
\end{equation}
where $s_z=1$ in non-PML region and $s_x=\kappa_z+\frac{\sigma_z}{\alpha_z+j\omega\epsilon_0}$ in PML region.
Transform to time domain we get
\begin{equation}
\frac{\partial( \epsilon E_{x})}{\partial t}+\sigma E_{x}=-\frac{1}{\kappa_{z}}\frac{\partial H_{y}}{\partial z}-\Psi_{Ezy}
\end{equation}
\begin{equation}
\frac{\partial( \mu H_{y})}{\partial t}+\sigma_{m} H_{y}=\frac{1}{\kappa_{z}}\frac{\partial E_{x}}{\partial z}+\Psi_{Hzx}
\end{equation}
Here
\begin{equation}
\Psi_{Ezy}=\zeta_{z}(t)*\frac{\partial H_{y}}{\partial z}
\end{equation}
and
\begin{equation}
\Psi_{Hzx}=\zeta_{z}(t)*\frac{\partial E_{x}}{\partial z}
\end{equation}
where
\begin{equation}
\zeta_{z}(t)=-\frac{\sigma_z}{\epsilon_0\kappa^{2}_{z}}\exp\left(-\left(\frac{\sigma_z}{\epsilon_0\kappa_z}+\frac{\alpha_z}{\epsilon_0}\right)t\right)u(t)
\end{equation}
and $u(t)$ is the unit step function.

\section{Discrete formula}
%%=========================================
%% electric dicrete equation
%%=========================================
\begin{equation}
\begin{aligned}
&\epsilon(k)\frac{E^{n+1}_{x}(k)-E^{n}_{x}(k)}{\Delta t}+\sigma(k)\frac{E^{n+1}_{x}(k)+E^{n}_{x}(k)}{2}=\\
&-\frac{1}{\kappa_z(k)}\frac{H^{n+1/2}_{y}(k+1/2)-H^{n+1/2}_{y}(k-1/2)}{\Delta z}-\Psi_{Ezy}^{n+1/2}(k)
\end{aligned}
\end{equation}
\begin{equation}
\begin{aligned}
&E^{n+1}_{x}(k)=C_{a}(k)E^{n}_{x}(k)\\
&+C_{b}(k)\left(H^{n+1/2}_{y}(k+1/2)-H^{n+1/2}_{y}(k-1/2)\right)+C_{c}(k)\Psi_{Ezy}^{n+1/2}(k)
\end{aligned}
\end{equation}
where 
\begin{equation}
C_{a}(k)=\frac{1-b}{1+b}
\end{equation}
\begin{equation}
C_{c}(k)=-\frac{\Delta t}{(1+b)\epsilon(k)}
\end{equation}
\begin{equation}
C_{b}(k)=\frac{C_{c}}{\kappa(k)\Delta z}
\end{equation}
\begin{equation}
b=\frac{\sigma(k)\Delta t}{2\epsilon(k)}
\end{equation}

%%=========================================
%% magnetic dicrete equation
%%=========================================
Magnetic
\begin{equation}
\begin{aligned}
&\mu(k)\frac{H^{n+1/2}_{y}(k+1/2)-H^{n+1/2}_{y}(k+1/2)}{\Delta t}\\
&+\sigma_m(k)\frac{H^{n+1/2}_{x}(k)+H^{n-1/2}_{x}(k+1/2)}{2}=\\
&\frac{1}{\kappa_z(k)}\frac{E^{n}_{x}(k+1)-E^{n}_{x}(k)}{\Delta z}-\Psi_{Hzx}^{n+1/2}(k+1/2)
\end{aligned}
\end{equation}
\begin{equation}
\begin{aligned}
&H^{n+1/2}_{y}(k+1/2)=C_{1}(k+1/2)H^{n-1/2}_{y}(k+1/2)\\
&+C_{2}(k+1/2)\left(E^{n}_{x}(k+1)-E^{n}_{x}(k)\right)+C_{3}(k+1/2)\Psi_{Hzx}^{n}(k+1/2)
\end{aligned}
\end{equation}
where 
\begin{equation}
C_{1}(k)=\frac{1-b}{1+b}
\end{equation}
\begin{equation}
C_{3}(k)=\frac{\Delta t}{(1+b)\mu(k)}
\end{equation}
\begin{equation}
C_{2}(k)=\frac{C_{3}}{\kappa(k)\Delta z}
\end{equation}
\begin{equation}
b=\frac{\sigma_m(k)\Delta t}{2\mu(k)}
\end{equation}
\end{document}
